C0deine/Type/SyntaxTree/Anno.lean
@@ -11,31 +11,31 @@ open Typ
 
 open Typ.Notation in
 inductive Anno (Δ : GCtx) (Γ : FCtx) : Type
-| requires   : {τ : {τ : Typ // τ = (bool)}} → Expr.NoResult Δ Γ τ → Anno Δ Γ
-| ensures    : {τ : {τ : Typ // τ = (bool)}} → Expr          Δ Γ τ → Anno Δ Γ
-| loop_invar : {τ : {τ : Typ // τ = (bool)}} → Expr.NoResult Δ Γ τ → Anno Δ Γ
-| assert     : {τ : {τ : Typ // τ = (bool)}} → Expr.NoResult Δ Γ τ → Anno Δ Γ
+| requires   : τ = (bool) → Expr.NoResult Δ Γ τ → Anno Δ Γ
+| ensures    : τ = (bool) → Expr          Δ Γ τ → Anno Δ Γ
+| loop_invar : τ = (bool) → Expr.NoResult Δ Γ τ → Anno Δ Γ
+| assert     : τ = (bool) → Expr.NoResult Δ Γ τ → Anno Δ Γ
 
 -- only requires/ensures can annotate functions
 @[inline, reducible] def Anno.function : Anno Δ Γ → Bool
-  | .requires _   => true
-  | .ensures _    => true
-  | .loop_invar _ => false
-  | .assert _     => false
+  | .requires _ _   => true
+  | .ensures _ _    => true
+  | .loop_invar _ _ => false
+  | .assert _ _     => false
 
 -- only loop_invariant and assert can annotate loops
 @[inline, reducible] def Anno.loop : Anno Δ Γ  → Bool
-  | .requires _   => false
-  | .ensures _    => false
-  | .loop_invar _ => true
-  | .assert _     => false -- see language deviation
+  | .requires _ _   => false
+  | .ensures _ _    => false
+  | .loop_invar _ _ => true
+  | .assert _ _     => false -- see language deviation
 
 -- only assert can be not attatched to a loop/function
 @[inline, reducible] def Anno.free : Anno Δ Γ  → Bool
-  | .requires _   => false
-  | .ensures _    => false
-  | .loop_invar _ => false
-  | .assert _     => true
+  | .requires _ _   => false
+  | .ensures _ _    => false
+  | .loop_invar _ _ => false
+  | .assert _ _     => true
 
 abbrev Anno.Loop     Δ Γ := {a : Anno Δ Γ  // Anno.loop     a}
 abbrev Anno.Function Δ Γ := {a : Anno Δ Γ  // Anno.function a}
@@ -48,28 +48,28 @@ inductive Anno.Fold
     → α → Anno Δ Γ → α → Prop
 | requires
   : {a₁ a₂ : α}
-  → {τ : {τ : Typ // τ = (bool)}}
+  → {hτ : τ = (bool)}
   → {e : Expr.NoResult Δ Γ τ}
   → Expr.Fold P a₁ e.val a₂
-  → Anno.Fold P a₁ (.requires e) a₂
+  → Anno.Fold P a₁ (.requires hτ e) a₂
 | ensures
   : {a₁ a₂ : α}
-  → {τ : {τ : Typ // τ = (bool)}}
+  → {hτ : τ = (bool)}
   → {e : Expr Δ Γ τ}
   → Expr.Fold P a₁ e a₂
-  → Anno.Fold P a₁ (.ensures e) a₂
+  → Anno.Fold P a₁ (.ensures hτ e) a₂
 | loop_invar
   : {a₁ a₂ : α}
-  → {τ : {τ : Typ // τ = (bool)}}
+  → {hτ : τ = (bool)}
   → {e : Expr.NoResult Δ Γ τ}
   → Expr.Fold P a₁ e.val a₂
-  → Anno.Fold P a₁ (.loop_invar e) a₂
+  → Anno.Fold P a₁ (.loop_invar hτ e) a₂
 | assert
   : {a₁ a₂ : α}
-  → {τ : {τ : Typ // τ = (bool)}}
+  → {hτ : τ = (bool)}
   → {e : Expr.NoResult Δ Γ τ}
   → Expr.Fold P a₁ e.val a₂
-  → Anno.Fold P a₁ (.assert e) a₂
+  → Anno.Fold P a₁ (.assert hτ e) a₂
 
 inductive Anno.List.Fold
     : (P : (τ : Typ) → α → Expr Δ Γ τ → Option α)
@@ -81,10 +81,10 @@ inductive Anno.List.Fold
   → Anno.List.Fold P a₁ (anno :: annos) a₃
 
 def Anno.toString : Anno Δ Γ → String
-  | .requires e   => s!"//@requires {e}"
-  | .ensures e    => s!"//@ensures {e}"
-  | .loop_invar e => s!"//@loop_invariant {e}"
-  | .assert e     => s!"//@assert {e}"
+  | .requires _ e   => s!"//@requires {e}"
+  | .ensures _ e    => s!"//@ensures {e}"
+  | .loop_invar _ e => s!"//@loop_invariant {e}"
+  | .assert _ e     => s!"//@assert {e}"
 instance : ToString (Anno Δ Γ) := ⟨Anno.toString⟩
 def Anno.listToString : List (Anno Δ Γ) → String
   | [] => ""
