C0deine/Type/SyntaxTree/Dynamics/Determinism.lean
@@ -7,7 +7,64 @@ import C0deine.Type.SyntaxTree.Dynamics.Step
 
 namespace C0deine.Tst.Dynamics
 
+theorem Step.UnOp.deterministic {op : Tst.UnOp} {v v₁ v₂ : Value}
+    (h₁ : Step.UnOp op v v₁) (h₂ : Step.UnOp op v v₂) : v₁ = v₂ := by
+  cases h₁ <;> (cases h₂; rfl)
+
+theorem Step.BinOp.Int.deterministic {op : Tst.BinOp.Int} {v₁ v₂ : Value}
+    (h₁ : Step.BinOp.Int v₁ op v₂ r₁)
+    (h₂ : Step.BinOp.Int v₁ op v₂ r₂)
+    : r₁ = r₂ := by
+  cases h₁ <;> (cases h₂; rfl)
+
+theorem Step.BinOp.Cmp.deterministic {op : Comparator} {v₁ v₂ : Value}
+    (h₁ : Step.BinOp.Cmp v₁ op v₂ r₁)
+    (h₂ : Step.BinOp.Cmp v₁ op v₂ r₂)
+    : r₁ = r₂ := by
+  cases h₁ <;> (cases h₂; rfl)
+
+
+theorem Step.State.mk_iff_result_eq {p : Prog} {r₁ r₂ : DynResult} :
+    r₁ = r₂ ↔ State.mk (p := p) H S η r₁ = State.mk H S η r₂ := by
+  apply Iff.intro <;> intro h₁
+  . simp only [State.mk.injEq, DynResult.val.injEq, true_and, h₁]
+  . simp only [State.mk.injEq, true_and] at h₁
+    exact h₁
+
+
+theorem Step.val_deterministic {p : Prog} {s₁ s₂ : State p}
+    (h₁ : Step { H := H, S := S, η := η, r := DynResult.val v K } s₁)
+    (h₂ : Step { H := H, S := S, η := η, r := DynResult.val v K } s₂)
+    : s₁ = s₂ := by
+  cases h₁ <;> cases h₂ <;> try (
+    apply Step.State.mk_iff_result_eq.mp
+    simp
+    first
+    | exact Step.UnOp.deterministic (by assumption) (by assumption)
+    | exact Sum.inl.inj (Step.BinOp.Int.deterministic (by assumption) (by assumption))
+    | exact Sum.inr.inj (Step.BinOp.Int.deterministic (by assumption) (by assumption))
+    | exact Step.BinOp.Cmp.deterministic (by assumption) (by assumption)
+    | next h' _exn h'' =>
+        have := Step.BinOp.Int.deterministic h' h''
+        contradiction
+    | skip
+  )
+  all_goals sorry
+
+theorem Step.eval_deterministic {p : Prog} {s₁ s₂ : State p}
+    (h₁ : Step { H := H, S := S, η := η, r := DynResult.eval e K } s₁)
+    (h₂ : Step { H := H, S := S, η := η, r := DynResult.eval e K } s₂)
+    : s₁ = s₂ := by
+  sorry
 
 theorem Step.deterministic {p : Prog} {s s₁ s₂ : State p}
     (h₁ : Step s s₁) (h₂ : Step s s₂) : s₁ = s₂ := by
-  sorry
+  let ⟨H, S, η, r⟩ := s
+  cases r
+  case val Δ Γ τ v K     => exact Step.val_deterministic h₁ h₂
+  case eval Δ Γ τ rk e K => exact Step.eval_deterministic h₁ h₂
+  case exec Δ Γ ρ rk s K => sorry
+  case exec_seq          => cases h₁
+  case exn               => cases h₁
+  case nop               => cases h₁
+  case res               => cases h₁
