C0deine/Type/SyntaxTree/LValue.lean
@@ -14,17 +14,17 @@ inductive LValue (Δ : GCtx) (Γ : FCtx) : Typ → Type
 | var   : (x : Symbol)
         → (Γ.syms x = .some (.var τ))
         → LValue Δ Γ τ
-| dot   : {τ₁ : {τ : Typ // τ = (struct s)}}
+| dot   : (hτ₁ : τ₁ = (struct s))
         → LValue Δ Γ τ₁
         → (field : Symbol)
         → Δ.struct s = .some ⟨fields, true⟩
         → fields field = .some τ
         → LValue Δ Γ τ
-| deref : {τ₁ : {τ' : Typ // τ' = (τ*)}}
+| deref : (hτ₁ : τ₁ = (τ*))
         → LValue Δ Γ τ₁
         → LValue Δ Γ τ
-| index : {τ₁ : {τ' : Typ // τ' = (τ[])}}
-        → {τ₂ : {τ : Typ // τ = (int)}}
+| index : (hτ₁ : τ₁ = (τ[]))
+        → (hτ₂ : τ₂ = (int))
         → LValue Δ Γ τ₁
         → Expr.NoContract Δ Γ τ₂
         → LValue Δ Γ τ
@@ -38,25 +38,11 @@ open Typ.Notation
 @[inline] def get_name
     (lval : LValue Δ Γ τ) (h₁ : lval.is_var) : Symbol :=
   match h₂ : lval with
-  | .var name _   => name
-  | .dot _ _ _ _
-  | .deref _
-  | .index _ _    => by simp [is_var] at h₁
+  | .var name _       => name
+  | .dot _ _ _ _ _
+  | .deref _ _
+  | .index _ _ _ _    => by simp [is_var] at h₁
 
-@[inline] def typeWith {p : Typ → Prop} (e : LValue Δ Γ τ) (h : p τ)
-    : LValue Δ Γ (⟨τ, h⟩ : {τ : Typ // p τ}) := e
-@[inline] def typeWithEq {τ₂ : Typ} (e : LValue Δ Γ τ) (eq : τ = τ₂)
-    : LValue Δ Γ (⟨τ, eq⟩ : {τ : Typ // τ = τ₂}) :=
-  e.typeWith (p := fun t => t = τ₂) eq
-
-@[inline] def intType (e : LValue Δ Γ τ) (eq : τ = (int))
-    : LValue Δ Γ (⟨τ, eq⟩ : {τ : Typ // τ = (int)}) := e.typeWithEq eq
-@[inline] def ptrType (e : LValue Δ Γ τ) (τ' : Typ) (eq : τ = (τ'*))
-    : LValue Δ Γ (⟨τ, eq⟩ : {τ : Typ // τ = (τ'*)}) := e.typeWithEq eq
-@[inline] def arrType (e : LValue Δ Γ τ) (τ' : Typ) (eq : τ = (τ'[]))
-    : LValue Δ Γ (⟨τ, eq⟩ : {τ : Typ // τ = (τ'[])}) := e.typeWithEq eq
-@[inline] def structType (e : LValue Δ Γ τ) (s : Symbol) (eq : τ = (struct s))
-    : LValue Δ Γ (⟨τ, eq⟩ : {τ : Typ // τ = (struct s)}) := e.typeWithEq eq
 
 structure Predicate (Δ : GCtx) (Γ : FCtx) (α : Type) where
   lval : (τ : Typ) → α → LValue Δ Γ τ → Option α
@@ -72,33 +58,39 @@ inductive Fold : {Δ : GCtx} → {Γ : FCtx}
   → P.lval _ a₁ (.var x h) = some a₂
   → Fold P a₁ ((.var x h) : LValue Δ Γ _) a₂
 | dot
-  : Fold P a₁ l a₂
-  → P.lval _ a₂ (.dot l f h₁ h₂) = some a₃
-  → Fold P a₁ (.dot l f h₁ h₂) a₃
+  : {a₁ a₂ : α}
+  → {hτ₁ : τ₁ = (struct s)}
+  → Fold P a₁ l a₂
+  → P.lval _ a₂ (.dot hτ₁ l f h₁ h₂) = some a₃
+  → Fold P a₁ (.dot hτ₁ l f h₁ h₂) a₃
 | deref
-  : Fold P a₁ l a₂
-  → P.lval _ a₂ (.deref l) = some a₃
-  → Fold P a₁ (.deref l) a₃
+  : {hτ₁ : τ₁ = (τ*)}
+  → Fold P a₁ l a₂
+  → P.lval _ a₂ (.deref hτ₁ l) = some a₃
+  → Fold P a₁ (.deref hτ₁ l) a₃
 | index
-  : Fold P a₁ l a₂
+  : {hτ₁ : τ₁ = (τ[])}
+  → {hτ₂ : τ₂ = (int)}
+  → {l : LValue Δ Γ τ₁}
+  → Fold P a₁ l a₂
   → Expr.Fold P.expr a₂ e.val a₃
-  → P.lval _ a₃ (.index l e) = some a₄
-  → Fold P a₁ (.index l e) a₄
+  → P.lval _ a₃ (.index hτ₁ hτ₂ l e) = some a₄
+  → Fold P a₁ (.index hτ₁ hτ₂ l e) a₄
 
 def toExpr {τ : Typ} : LValue Δ Γ τ → Expr Δ Γ τ
   | .var x h        => .var x h
-  | .dot lv f h₁ h₂ => .dot lv.toExpr f h₁ h₂
-  | .deref lv       => .deref lv.toExpr
-  | .index lv ind   => .index lv.toExpr ind.val
+  | .dot hτ₁ lv f h₁ h₂ => .dot hτ₁ lv.toExpr f h₁ h₂
+  | .deref hτ₁ lv       => .deref hτ₁ lv.toExpr
+  | .index hτ₁ hτ₂ lv ind   =>
+    .index hτ₁ hτ₂ lv.toExpr ind.val
 
 end LValue
 
 def LValue.toString : LValue Δ Γ τ → String
-  | .var name _ => s!"({name} : {τ})"
-  | .dot e field _ _ =>
-    s!"({LValue.toString e}.{field} : {τ})"
-  | .deref e => s!"(*{LValue.toString e} : {τ})"
-  | .index e i => s!"({LValue.toString e}[{i}] : {τ})"
+  | .var name _        => s!"({name} : {τ})"
+  | .dot _ e field _ _ => s!"({LValue.toString e}.{field} : {τ})"
+  | .deref _ e         => s!"(*{LValue.toString e} : {τ})"
+  | .index _ _ e i     => s!"({LValue.toString e}[{i}] : {τ})"
 
 instance : ToString (LValue Δ Γ τ) where toString := LValue.toString
 instance : ToString (List (Typed Symbol)) where
